examples/QueryStructure/Bookstore.v
@@ -104,7 +104,7 @@ Proof.
 (* <130 seconds for master_plan.
    <141 seconds for Defined. *)
 
-Time Definition BookstoreImpl' : SharpenedUnderDelegates BookstoreSig :=
-  Eval cbv beta delta iota in projT1 SharpenedBookStore.
+Time Definition BookstoreImpl' : SharpenedUnderDelegates BookStoreSig :=
+  Eval simpl in projT1 SharpenedBookStore.
 
 Print BookstoreImpl'.
